wip: linearization

src/spec/Flutterbye.Linearization.fst
@@ -28,59 +28,55 @@ type step_t 'a =
    | Stale: op:('a -> Tot 'a) -> step_t 'a
 
 type contains_commit_p (#a_t:Type) (steps:seq (step_t a_t)) =
-   exists (x:nat{x < length steps}).
-      is_Commit (index steps x)
+   length steps > 0
+   /\ (exists (x:nat{x < length steps}).
+         is_Commit (index steps x))
 
-type contains_fresh_p (#a_t:Type) (pending:seq (pending_t a_t)) (state:a_t) = 
-   exists (x:nat{x < length pending}).
-      Pending.observed (index pending x) = state
+type contains_fresh_p (#a_t:Type) (pending:seq (pending_t a_t)) (state:a_t) =
+   length pending > 0
+   /\ (exists (x:nat{x < length pending}).
+         Pending.observed (index pending x) = state)
 
-(*type advance_loop_p: 
-   #a_t:Type 
-   -> pending0:seq (pending_t xns)
-   -> state:a_t                                       
-   -> pending:seq (pending_t xns)
-   -> steps:seq (step_t xns)      
-   -> Type
-= fun #a_t xns pending0 state pending steps ->
-      (length pending0 <= length xns)
-      /\ (length pending <= length pending0)
-      /\ (contains_commit_p xns steps
-         \/ contains_fresh_p xns pending state)*)
+(*type advance_loop_invariants_p 
+   (#a_t:Type) 
+   (pending0:seq (pending_t a_t)) 
+   (pending:seq (pending_t a_t))
+   (state:'a)
+   (steps:seq (step_t a_t))
+=     (length pending <= length pending0)
+   /\ (contains_commit_p steps \/ contains_fresh_p pending state)*)
 
 val advance_loop:
-      pending0:seq (pending_t 'a)
-   -> pending:seq (pending_t 'a)
+      pending:seq (pending_t 'a)
    -> state:'a
-   -> steps:seq (step_t 'a)
-   -> Tot (steps':seq (step_t 'a))
+   -> steps:seq (step_t 'a){contains_commit_p steps \/ contains_fresh_p pending state}
+   -> Tot (steps':seq (step_t 'a){contains_commit_p steps'})
       (decreases (length pending))
-let rec advance_loop pending0 pending state steps =
+let rec advance_loop pending state steps =
    if 0 = length pending then
       steps
    else begin
       let i = 0 in
       let p = index pending i in
-      let fresh = (Pending.observed p = state) in
       let op = Pending.op p in
-      let step' =
-         if fresh then
-            Commit op
-         else
-            Stale op
-      in
-      let state' =
-         if fresh then
-            op state
-         else
-            state
-      in
-      let steps' = append steps (create 1 step') in
-      let pending' = remove pending i in
-      advance_loop pending0 pending' state' steps'
+      let fresh = (Pending.observed p = state) in
+      if fresh then begin
+         admit ();
+         let step' = Commit op in
+         let state' = op state in
+         let steps' = append steps (create 1 step') in
+         let pending' = remove pending i in
+         advance_loop pending' state' steps'
+      end else begin
+         admit ();
+         let step' = Stale op in
+         let steps' = append steps (create 1 step') in
+         let pending' = remove pending i in
+         advance_loop pending' state steps'
+      end         
    end
 
-val advance_loop_lemma:
+(*val advance_loop_lemma:
       pending0:seq (pending_t 'a)
    -> pending:seq (pending_t 'a)
    -> state:'a
@@ -112,7 +108,7 @@ let rec advance_loop_lemma pending0 pending state steps =
       let steps' = append steps (create 1 step') in
       let pending' = remove pending i in
       advance_loop_lemma pending0 pending' state' steps'
-   end
+   end*)
 
 (*type advanced_p (pending:seq (pending_t 'a)) (state:'a) (steps:seq (step_t 'a)) =
    length pending <= length xns
